LeanMenhir.lean
@@ -19,6 +19,7 @@ import LeanMenhir.Guarantees
 import LeanMenhir.Generator.FinAlphabet
 import LeanMenhir.Generator.Tables
 import LeanMenhir.Generator.Grammar0
+import LeanMenhir.Generator.Derives0
 import LeanMenhir.Generator.LR1
 import LeanMenhir.Generator.BuildTables
 import LeanMenhir.Generator.GrammarCheck
